\documentclass{tikzcd}

\begin{document}
  \begin{tikzcd}
      &                                                    & E \ar[d, "E \to (E + E)"]                                &   \\
      &                                                    & (E + E) \ar[ld, "E \to (E + E)" swap] \ar[rd, "E \to 3"] &   \\
      & (E + E) \ar[ld, "E \to 1" swap] \ar[rd, "E \to 2"] &                                                          & 3 \\
    1 &                                                    & 2                                                        &
  \end{tikzcd}

  \begin{tikzcd}
      &                                                  & E \ar[d, "E \to E + E"]                              &   \\
      &                                                  & E + E \ar[ld, "E \to E + E" swap] \ar[rd, "E \to 3"] &   \\
      & E + E \ar[ld, "E \to 1" swap] \ar[rd, "E \to 2"] &                                                      & 3 \\
    1 &                                                  & 2                                                    &
  \end{tikzcd}

  \begin{tikzcd}
      & E \ar[d, "E \to E + E"]                              &                                                   &   \\
      & E + E \ar[ld, "E \to 1" swap] \ar[rd, "E \to E + E"] &                                                   &   \\
    1 &                                                      & E + E \ar[ld, "E \to 2"' swap] \ar[rd, "E \to 3"] &   \\
      & 2                                                    &                                                   & 3
  \end{tikzcd}
\end{document}
